src/compiler_generic/toy_example/embedding/meta_toy/Meta_META.thy
@@ -58,6 +58,13 @@ text\<open>Most of the Meta-Model we have defined (in particular those defined i
 
 datatype toy_flush_all = ToyFlushAll
 
+subsection\<open>The Generic Meta-Model\<close>
+
+text\<open>The generic Meta-Model can simulate any other Meta-Models \<open>M\<close> by taking a string representing
+     some ML code, which is supposed to express a parsed value inhabiting \<open>M\<close>.\<close>
+
+datatype toy_generic = ToyGeneric string
+
 subsection\<open>The META Meta-Model (I)\<close>
 
 datatype floor = Floor1 | Floor2 | Floor3 (* NOTE nat can be used *)
@@ -93,6 +100,7 @@ datatype all_meta_embedding = META_enum toy_enum
                             | META_def_transition floor toy_def_transition
                             | META_class_tree toy_class_tree
                             | META_flush_all toy_flush_all
+                            | META_generic toy_generic
 
 subsection\<open>Main Compiling Environment\<close>
 
@@ -195,7 +203,11 @@ datatype all_meta = (* pure Isabelle *)
 
 text\<open>As remark, the Isabelle Meta-Model represented by @{typ semi__theories} can be merged
 with the previous META Meta-Model @{typ all_meta_embedding}.
-However a corresponding parser and printer would then be required.\<close>
+However a corresponding parser and printer would then be required, instead we can just regroup them
+in a temporary type:\<close>
+
+datatype fold_all_input = Fold_meta all_meta_embedding
+                        | Fold_custom "all_meta list"
 
 subsubsection\<open>Extending the Meta-Model\<close>
 
